In progress epoch correctness

high/Veritas.Verifier.Correctness.fst
@@ -29,8 +29,8 @@ module TL = Veritas.Verifier.TSLog
 #push-options "--max_fuel 1 --max_ifuel 1 --initial_fuel 1 --initial_ifuel 1"
 
 (* state ops of all vlogs of all verifier threads upto epoch ep *)
-let to_state_op_gvlog (gl: g_vlog) (ep: epoch) =
-  map to_state_op_vlog (map prefix_upto_epoch ep) gl
+let to_state_op_gvlog (gl: g_vlog) =
+  map to_state_op_vlog gl
 
 let lemma_vlog_interleave_implies_state_ops_interleave (l: vlog) (gl: g_vlog{interleave #vlog_entry l gl})
   : Lemma (interleave #state_op (to_state_op_vlog l) (to_state_op_gvlog gl)) 
@@ -42,48 +42,58 @@ let lemma_vlog_interleave_implies_state_ops_interleave (l: vlog) (gl: g_vlog{int
         let i' = Veritas.Interleave.filter_map_interleaving is_state_op to_state_op i in
         FStar.Squash.return_squash i')
 
-let lemma_time_seq_rw_consistent  
-  (itsl: TL.hash_verifiable_log {~ (rw_consistent (state_ops itsl))})
-  : hash_collision_gen = 
-  let tsl = i_seq itsl in  
-  let ts_ops = to_state_op_vlog tsl in
-  
-  //assert(~ (rw_consistent ts_ops));
+let lemma_time_seq_rw_consistent
+  (epmax: epoch)
+  (itsl: TL.hash_verifiable_log epmax {
+    let itsl_ep = prefix_upto_epoch epmax itsl in
+    ~ (rw_consistent (state_ops itsl_ep))})
+  : hash_collision_gen =
 
-  if TL.is_eac itsl then (
+  let itsl_ep = prefix_upto_epoch epmax itsl in
+  let ts_ops = state_ops itsl_ep in
+  assert(~ (rw_consistent ts_ops));
+
+  if TL.is_eac itsl_ep then (
     // ts log is eac implies state ops in that sequence are rw-consistent
-    TL.lemma_eac_implies_state_ops_rw_consistent itsl;
-
+    TL.lemma_eac_implies_state_ops_rw_consistent itsl_ep;
     // ... which is a contradiction
-    //assert(rw_consistent ts_ops);
-
+    assert(rw_consistent ts_ops);
     (* any return value *)
     SingleHashCollision (Collision (DVal Null) (DVal Null))
   )
   else
-    lemma_non_eac_time_seq_implies_hash_collision itsl
+    lemma_non_eac_time_seq_implies_hash_collision epmax itsl
 
 (* final verifier correctness theorem *)
-let lemma_verifier_correct (gl: VG.hash_verifiable_log { ~ (seq_consistent (to_state_op_gvlog gl))}):
-  hash_collision_gen =    
-  (* sequences of per-thread put/get operations *)
-  let g_ops = to_state_op_gvlog gl in
+let lemma_verifier_correct
+  (epmax: epoch)
+  (gl: VG.hash_verifiable_log epmax { ~ (seq_consistent (to_state_op_gvlog (VG.prefix_upto_epoch epmax gl)))}):
+  hash_collision_gen =
+
+  (* log entries upto epoch epmax *)
+  let gl_ep = VG.prefix_upto_epoch epmax gl in
+
+  (* state ops in the first epmax epochs *)
+  let g_ops = to_state_op_gvlog gl_ep in
 
   (* sequence ordered by time of each log entry *)
-  let itsl = TL.create gl in  
-  lemma_interleaving_correct itsl;
-  assert(interleave (i_seq itsl) gl);
+  let itsl = TL.create gl in
 
-  (* sequence of state ops induced by tmsl *)
-  let ts_ops = state_ops itsl in
+  (* log entries upto epoch epmax *)
+  let itsl_ep = prefix_upto_epoch epmax itsl in
+  assert(gl_ep = g_vlog_of itsl_ep);
+  lemma_interleaving_correct itsl_ep;
+  assert(interleave (i_seq itsl_ep) gl_ep);
 
-  lemma_vlog_interleave_implies_state_ops_interleave (i_seq itsl) gl;
+  (* sequence of state ops projected from time ordered sequence *)
+  let ts_ops = state_ops itsl_ep in
+  lemma_vlog_interleave_implies_state_ops_interleave (i_seq itsl_ep) gl_ep;
   assert(interleave ts_ops g_ops);
 
   (* if tm_ops is read-write consistent then we have a contradiction *)
   let is_rw_consistent = valid_all_comp ssm ts_ops in
   lemma_state_sm_equiv_rw_consistent ts_ops;
-  
+
   if is_rw_consistent then (
     assert(valid_all ssm ts_ops);
     assert(rw_consistent ts_ops);
@@ -94,8 +104,5 @@ let lemma_verifier_correct (gl: VG.hash_verifiable_log { ~ (seq_consistent (to_s
     (* any return value *)
     SingleHashCollision (Collision (DVal Null) (DVal Null))
   )
-  else  
-    //assert(~ (rw_consistent ts_ops));
-    lemma_time_seq_rw_consistent itsl
-  
-
+  else
+    lemma_time_seq_rw_consistent epmax itsl
